\documentclass[12pt, letterpaper, onecolumn, conference, final]{IEEEtran}

\usepackage[margin = .5in]{geometry}
\usepackage{amsmath}
\usepackage{amsthm}
\usepackage{amssymb}
\usepackage{wasysym}
\usepackage{graphicx}
\usepackage{mathtools}
\usepackage{cancel}

\title{Project Euler: Problem 6 Personal Comments}
\author{Nathan Marianovsky}

\newcommand{\Mod}[1]{\ (\text{mod}\ #1)}

\theoremstyle{definition}
\newtheorem*{problem*}{Problem}
\newtheorem*{solution*}{Solution}

\theoremstyle{plain}

\renewcommand\thesection{\arabic{section}}

\begin{document}

\maketitle

\section*{\underline{\Large{Sum of First $n$ Natural Numbers}}}
\vspace{.3cm}
\noindent
To derive the formula for finding the sum of the first $n$ natural numbers consider the following:
\begin{equation*}
\begin{split}
s_n = 1 + 2 + 3 + \dots + (n-2) + (n-1) + n \\
s_n = n + (n-1) + (n-2) + \dots + 3 + 2 + 1
\end{split}
\end{equation*}
The second line is just the first rewritten backwards. Now add the two equations:
\begin{equation*}
2s_n = n(n+1)
\end{equation*}
which yields the final formula:
\begin{equation*}
s_n = \frac{n(n+1)}{2} = \sum_{i=1}^n i
\end{equation*}

\vspace{.3cm}
\section*{\underline{\Large{Sum of Squares of First $n$ Natural Numbers}}}
\vspace{.3cm}
\noindent
Consider the following telescoping series:
\begin{equation*}
\sum_{i=1}^n ((1+i)^3 - i^3) = (\cancel{2^3} - 1^3) + (\cancel{3^3} - \cancel{2^3}) + (\cancel{4^3} - \cancel{3^3}) + \dots + (\cancel{n^3} - \cancel{(n-1)^3}) + ((n+1)^3 - \cancel{n^3}) = (n + 1)^3 - 1
\end{equation*}
On the other hand this summation can also be written as:
\begin{equation*}
\sum_{i=1}^n ((1+i)^3 - i^3) = \sum_{i=1}^n (i^3 + 3i^2 + 3i + 1 - i^3) = 3\sum_{i=1}^n i^2 + 3\sum_{i=1}^n i + n 
\end{equation*}
Now comparing both sides and solving for the sum of the squares gives:
\begin{equation*}
\begin{split}
3\sum_{i=1}^n i^2 + 3\sum_{i=1}^n i + n  &= (n + 1)^3 - 1 \\
\sum_{i=1}^n i^2 &= \frac{(n + 1)^3 - 1 - n}{3} - \sum_{i=1}^n i \\
\sum_{i=1}^n i^2 &= \frac{(n + 1)^3 - 1 - n}{3} - \frac{n(n + 1)}{2} \\
\sum_{i=1}^n i^2 &= \frac{n^3 + 3n^2 + 2n}{3} - \frac{n^2 + n}{2} \\
\sum_{i=1}^n i^2 &= \frac{n(n + 1)(2n + 1)}{6}
\end{split}
\end{equation*}



\end{document}